Must set characterization

theories/Testing_Pre_orders/Must/Alternative_Preorder/Must_Set/DefinitionMS.v
@@ -29,47 +29,55 @@ From Stdlib.Program Require Import Equality.
 From stdpp Require Import finite gmap decidable.
 
 From TestingTheory Require Import ActTau gLts Bisimulation Lts_OBA Subset_Act WeakTransitions Testing_Predicate
-    StateTransitionSystems InteractionBetweenLts Convergence Termination FiniteImageLTS.
+    StateTransitionSystems InteractionBetweenLts Convergence Termination FiniteImageLTS DefinitionAS.
 
-Section must_sets.
+(* https://arxiv.org/pdf/1612.03191.pdf *)
 
-  (* https://arxiv.org/pdf/1612.03191.pdf *)
+(* Local Open Scope positive. *)
 
-  Local Open Scope positive.
+Definition MUST `{
+  gLtsP : @gLts P A H, CC : Countable PreAct, @FinitaryAbsAction P T FinA PreAct A H Φ 𝝳 _ gLtsEqT _ _}
+  (p : P) (G : gset PreAct) :=
+  forall p', p ⟹ p' -> exists β p0, ( 𝝳 ∘ Φ ) β ∈ G /\ p' ⟹{co β} p0. (* /\ blocking β. *)
 
-  Definition MUST `{gLts P A}
-    (p : P) (G : gset A) :=
-    forall p', p ⟹ p' -> exists μ p0, μ ∈ G /\ p' ⟹{μ} p0.
+Definition MUST__s `{
+  gLtsP : @gLts P A H, !FiniteImagegLts P A,
+  CC : Countable PreAct, @FinitaryAbsAction P T FinA PreAct A H Φ 𝝳 _ gLtsEqT _ _ }
+  (ps : gset P) (G : gset PreAct) := 
+  forall p, p ∈ ps -> MUST p G.
 
-  Definition MUST__s `{FiniteImagegLts P A} 
-    (ps : gset P) (G : gset A) := 
-    forall p, p ∈ ps -> MUST p G.
+(* Residuals of a process p AFTER the execution of s. *)
 
-  (* Residuals of a process p AFTER the execution of s. *)
+Definition AFTER `{FiniteImagegLts P A} 
+  (p : P) (s : trace A) (hcnv : p ⇓ s) := 
+  wt_set p s hcnv.
 
-  Definition AFTER `{FiniteImagegLts P A} 
-    (p : P) (s : trace A) (hcnv : p ⇓ s) := 
-    wt_set p s hcnv. 
+Definition bhv_pre_ms_cond1 `{@gLts P A H, @gLts Q A H} 
+(p : P) (q : Q) := forall s, p ⇓ s -> q ⇓ s.
 
-  Definition bhv_pre_ms_cond1 `{gLts P A, gLts Q A} 
-  (p : P) (q : Q) := forall s, p ⇓ s -> q ⇓ s.
+Definition bhv_pre_ms_cond2 `{
+  gLtsP : @gLts P A H, !FiniteImagegLts P A, CC : Countable PreAct,
+  @FinitaryAbsAction P T FinA PreAct A H Φ 𝝳P _ gLtsEqT _ _,
+  gLtsQ : @gLts Q A H, !FiniteImagegLts Q A,
+  @FinitaryAbsAction Q T FinA PreAct A H Φ 𝝳Q _ gLtsEqT _ _}
+  (p : P) (q : Q) :=
+  forall s (hp : p ⇓ s) (hq : q ⇓ s) G, MUST__s (AFTER p s hp) G -> MUST__s (AFTER q s hq) G.
 
-  Definition bhv_pre_ms_cond2 `{@FiniteImagegLts P A H gLtsP, @FiniteImagegLts Q A H gLtsQ} 
-    (p : P) (q : Q) :=
-    forall s h1 h2 G, MUST__s (AFTER p s h1) G -> MUST__s (AFTER q s h2) G.
-
-  Definition bhv_pre_ms `{@FiniteImagegLts P A H gLtsP, @FiniteImagegLts Q A H gLtsQ} 
-    (p : P) (q : Q) :=
-    bhv_pre_ms_cond1 p q /\ bhv_pre_ms_cond2 p q.
-End must_sets.
+Definition bhv_pre_ms `{
+  gLtsP : @gLts P A H, !FiniteImagegLts P A, CC : Countable PreAct,
+  @FinitaryAbsAction P T FinA PreAct A H Φ 𝝳P _ gLtsEqT _ _,
+  gLtsQ : @gLts Q A H, !FiniteImagegLts Q A,
+  @FinitaryAbsAction Q T FinA PreAct A H Φ 𝝳Q _ gLtsEqT _ _}
+  (p : P) (q : Q) :=
+  bhv_pre_ms_cond1 p q /\ bhv_pre_ms_cond2 p q.
 
 Global Hint Unfold bhv_pre_ms:mdb.
 
 Notation "p 'MUST' G" := (MUST p G) (at level 70).
 
-Notation "p ≾₁ q" := (bhv_pre_ms_cond1 p q) (at level 70).
+Notation "p ₁≾ₘᵤₛₜ q" := (bhv_pre_ms_cond1 p q) (at level 70).
 
-Notation "p ≾₂ q" := (bhv_pre_ms_cond2 p q) (at level 70).
+Notation "p ₂≾ₘᵤₛₜ q" := (bhv_pre_ms_cond2 p q) (at level 70).
 
 Notation "p ≾ₘᵤₛₜ q" := (bhv_pre_ms p q) (at level 70).
 
