theories/Testing_Pre_orders/Must/Alternative_Preorder/Must_Set/Equivalence/EquivalenceMS.v
@@ -28,30 +28,50 @@ From Stdlib.Program Require Import Equality.
 
 From stdpp Require Import base decidable gmap finite.
 
-From TestingTheory Require Import gLts Bisimulation Lts_OBA Lts_FW Lts_OBA_FB StateTransitionSystems Termination
-    Must Bar Completeness Soundness Lift Subset_Act FiniteImageLTS WeakTransitions Convergence
-    InteractionBetweenLts MultisetLTSConstruction ForwarderConstruction ParallelLTSConstruction ActTau
-    Testing_Predicate DefinitionAS DefinitionMS MustE Equivalence.
+From TestingTheory Require Import 
+  gLts Lts_OBA Lts_OBA_FB Lts_FW FiniteImageLTS Lts_CN
+  Subset_Act ActTau 
+  Convergence Termination Bisimulation WeakTransitions
+  InteractionBetweenLts MultisetLTSConstruction 
+  ParallelLTSConstruction ForwarderConstruction
+  Testing_Predicate Must Lift DefinitionAS DefinitionMS
+  InFiniteSetHelper.
 
-Section must_set_acc_set.
-  Context `{P : Type}.
+Definition oas_all `{CC : Countable PreAct}  `{
+  gLtsP : @gLts P A H, FiniteImagegLts P A,
+  FiniteAbs : @FinitaryAbsAction P T FinA PreAct A H Φ 𝝳 gLtsP gLtsT _ _}
+  (p : P) (s : list A) (hcnv : p ⇓ s) : gset PreAct :=
+  let ps : list P := elements (wt_set p s hcnv) in
+  ⋃ map coR_abs ps.
+
+Definition oas `{CC : Countable PreAct}  `{
+  gLtsP : @gLts P A H, FiniteImagegLts P A,
+  FiniteAbs : @FinitaryAbsAction P T FinA PreAct A H Φ 𝝳 gLtsP gLtsT _ _}
+  (p : P) (s : list A) (hcnv : p ⇓ s) : gset PreAct :=
+  let ps : list P := elements (wt_refuses_set p s hcnv) in
+  ⋃ map coR_abs ps.
+
+(* From TestingTheory Require Import 
+    StateTransitionSystems DefinitionMS MustE Completeness Soundness Equivalence. *)
+
+
+(*   Context `{P : Type}.
   Context `{Q : Type}.
   Context `{A : Type}.
   Context `{H : !ExtAction A}.
 
-  Context `{@gLtsObaFB P A H gLtsEqP gLtsObaP, !FiniteImagegLts P A}.
-  Context `{@gLtsObaFB Q A H gLtsEqQ gLtsObaQ, !FiniteImagegLts Q A}.
+  Context `{@gLtsObaFW P A H gLtsEqP gLtsObaP, !FiniteImagegLts P A}.
+  Context `{@gLtsObaFW Q A H gLtsEqQ gLtsObaQ, !FiniteImagegLts Q A}.
+  Context `{gLtsT : @gLtsEq T A H}.
 
-  Context `{!Prop_of_Inter P (mb A) A fw_inter}.
-  Context `{!Prop_of_Inter Q (mb A) A fw_inter}.
-
-(*   Definition actions_acc 
-  (p : P * mb A) s (h : p ⇓ s) : gset PreA := oas p s h. *)
+  Context `{CC : Countable PreAct}.
+  Context `{@FinitaryAbsAction P T FinA PreAct A H Φ 𝝳 _ _ _ _ }.
+  Context `{@FinitaryAbsAction Q T FinA PreAct A H Φ 𝝳 _ _ _ _ }. *)
 
   (* ************************************************** *)
 
-  Lemma either_wperform_mu 
-  (p : P * mb A) μ :
+  Lemma either_wperform_mu `{gLts P A, !FiniteImagegLts P A}
+  (p : P) μ :
     p ⤓ -> (exists q, p ⟹{μ} q) \/ ~ (exists q, p ⟹{μ} q).
   Proof.
     intro ht. induction ht.
@@ -65,33 +85,36 @@ Section must_set_acc_set.
       + right. intros (q' & hw). inversion hw; subst.
         ++ contradict Hyp'. intros n. rewrite Forall_forall in n.
            eapply (n (dexist q l0)). eapply elem_of_enum. eauto.
-        ++ eapply (@lts_refuses_spec2 (P * mb A)); eauto.
+        ++ eapply (@lts_refuses_spec2 P); eauto.
     - left. eapply lts_refuses_spec1 in n as (q & l). eauto with mdb.
   Qed.
 
-  Lemma either_wperform_mem (p : P * mb A) (G : gset A) (ht : p ⤓) :
-    (exists μ p', μ ∈ G /\ p ⟹{μ} p') 
-      \/ (forall μ p', μ ∈ G -> ~ p ⟹{μ} p').
+  Lemma either_wperform_mem `{CC : Countable PreAct} `{gLts P A, !FiniteImagegLts P A} (Γ : A -> PreAct)
+    (p : P) (G : gset PreAct) (ht : p ⤓) :
+    (exists μ p', Γ μ ∈ G /\ p ⟹{co μ} p')
+      \/ (forall μ p', Γ μ ∈ G -> ~ p ⟹{co μ} p').
   Proof.
-    induction G using set_ind_L; [|destruct IHG, (either_wperform_mu p x)]; set_solver.
-  Qed.
+    (* induction G using set_ind_L; [|destruct IHG, (either_wperform_mu p (co x)]; set_solver. *)
+  Admitted.
 
-  Lemma either_wperform_mem_set
-    (ps : gset (P * mb A)) (G : gset A) (ht : forall p, p ∈ ps -> p ⤓) :
-    (exists p', p' ∈ ps /\ forall μ p0, μ ∈ G
-      -> ~ p' ⟹{μ} p0) 
-      \/ (forall p', p' ∈ ps -> exists μ p0, μ ∈ G /\ p' ⟹{μ} p0).
+  Lemma either_wperform_mem_set `{CC : Countable PreAct} `{@gLts P A H, !FiniteImagegLts P A}
+    `{@FinitaryAbsAction P T FinA PreAct A H Φ 𝝳 _ gLtsT _ _ }
+    (ps : gset P) (G : gset PreAct) (ht : forall p, p ∈ ps -> p ⤓) :
+    (exists p', p' ∈ ps /\ forall μ p0, ( 𝝳 ∘ Φ ) μ ∈ G
+      -> ~ p' ⟹{co μ} p0) 
+      \/ (forall p', p' ∈ ps -> exists μ p0, ( 𝝳 ∘ Φ ) μ ∈ G /\ p' ⟹{co μ} p0).
   Proof.
     induction ps using set_ind_L. 
     + set_solver. 
-    + destruct IHps, (@either_wperform_mem x G); set_solver.
+    + destruct IHps, (either_wperform_mem ( 𝝳 ∘ Φ ) x G); set_solver.
   Qed.
 
-  Lemma either_MUST
-      (p : P * mb A) (G : gset A) (hcnv : p ⇓ []) :
+  Lemma either_MUST `{CC : Countable PreAct} `{@gLts P A H, !FiniteImagegLts P A}
+      `{@FinitaryAbsAction P T FinA PreAct A H Φ 𝝳 _ gLtsT _ _ }
+      (p : P) (G : gset PreAct) (hcnv : p ⇓ []) :
       p MUST G \/ ~ p MUST G.
   Proof.
-    assert (∀ p0 : P * mb A, p0 ∈ wt_set p [] hcnv → p0 ⤓) as pre_Hyp.
+    assert (∀ p0 : P, p0 ∈ wt_set p [] hcnv → p0 ⤓) as pre_Hyp.
     intros p0 mem0%wt_set_spec1. eapply cnv_terminate, cnv_preserved_by_wt_nil; eauto.
     destruct (either_wperform_mem_set (wt_set p [] hcnv) G) 
       as [Hyp|]; eauto.
@@ -99,8 +122,9 @@ Section must_set_acc_set.
     - left. intros p1 hw%(wt_set_spec2 _ p1 [] hcnv). set_solver.
   Qed.
 
-  Lemma either_ex_nMUST_or_MUST
-    (ps : gset (P * mb A)) (G : gset A)
+  Lemma either_ex_nMUST_or_MUST `{CC : Countable PreAct} `{@gLts P A H, !FiniteImagegLts P A}
+    `{@FinitaryAbsAction P T FinA PreAct A H Φ 𝝳 _ gLtsT _ _ }
+    (ps : gset P) (G : gset PreAct)
       (ht : forall p, p ∈ ps -> p ⇓ []) :
     (exists p, p ∈ ps /\ ~ p MUST G) 
       \/ (forall p, p ∈ ps -> p MUST G).
@@ -108,26 +132,29 @@ Section must_set_acc_set.
     induction ps using set_ind_L; [|edestruct IHps, (either_MUST x G)]; set_solver.
   Qed.
 
-  Lemma either_MUST__s
-    (ps : gset (P * mb A)) (G : gset A)  :
+  Lemma either_MUST__s `{CC : Countable PreAct} `{@gLts P A H, !FiniteImagegLts P A}
+    `{@FinitaryAbsAction P T FinA PreAct A H Φ 𝝳 _ gLtsT _ _ }
+    (ps : gset P) (G : gset PreAct)  :
     (forall p, p ∈ ps -> p ⇓ []) -> MUST__s ps G \/ ~ MUST__s ps G.
   Proof.
     intros. edestruct (either_ex_nMUST_or_MUST ps G) as [Hyp |]; eauto.
     right. intros hm. destruct Hyp as (p0 & mem0%hm & hnm). contradiction.
   Qed.
 
-  Lemma nMusts_ex
-    (ps : gset (P * mb A)) (G : gset A) :
+  Lemma nMusts_ex `{CC : Countable PreAct} `{@gLts P A H, !FiniteImagegLts P A}
+    `{@FinitaryAbsAction P T FinA PreAct A H Φ 𝝳 _ gLtsT _ _ }
+    (ps : gset P) (G : gset PreAct) :
     (forall p, p ∈ ps -> p ⇓ []) -> ~ MUST__s ps G 
     -> exists p, p ∈ ps /\ ~ p MUST G.
   Proof. intros. edestruct (either_ex_nMUST_or_MUST ps G); set_solver. Qed.
 
-  Lemma nMust_ex
-    (p : P * mb A) (G : gset A) (hcnv : p ⇓ []) 
+  Lemma nMust_ex `{CC : Countable PreAct} `{@gLts P A H, !FiniteImagegLts P A}
+    `{@FinitaryAbsAction P T FinA PreAct A H Φ 𝝳 _ gLtsT _ _ }
+    (p : P) (G : gset PreAct) (hcnv : p ⇓ []) 
     (hnm : ~ p MUST G) :
-    exists p', p ⟹ p' /\ forall μ p0, μ ∈ G -> ~ p' ⟹{μ} p0.
+    exists p', p ⟹ p' /\ forall μ p0, 𝝳 (Φ μ) ∈ G -> ~ p' ⟹{co μ} p0.
   Proof.
-    assert (∀ p0 : P * mb A, p0 ∈ wt_set p [] hcnv → p0 ⤓).
+    assert (∀ p0 : P, p0 ∈ wt_set p [] hcnv → p0 ⤓).
     intros p0 mem0%wt_set_spec1. eapply cnv_terminate, cnv_preserved_by_wt_nil; eauto.
     destruct (either_wperform_mem_set (wt_set p [] hcnv) G) as [Hyp|Hyp]; eauto.
     - destruct Hyp as (p' & mem'%wt_set_spec1 & nhw). set_solver.
@@ -135,7 +162,9 @@ Section must_set_acc_set.
   Qed.
 
   Lemma nMusts_nMust
-  (p : P * mb A) (G : gset A) (hcnv : p ⇓ []) 
+  `{CC : Countable PreAct} `{@gLts P A H, !FiniteImagegLts P A}
+  `{@FinitaryAbsAction P T FinA PreAct A H Φ 𝝳 _ gLtsT _ _ }
+  (p : P) (G : gset PreAct) (hcnv : p ⇓ []) 
   (hnm : ~ MUST__s (wt_set p [] hcnv) G) : 
   ¬ p MUST G.
   Proof.
@@ -143,47 +172,54 @@ Section must_set_acc_set.
     intros r hw. eapply hm. eapply wt_push_nil_left; eassumption.
   Qed.
 
-(*   Lemma nMust_out_acc_ex 
-
-    (p : P * mb A) pt G s hcnv :
+  Lemma nMust_out_acc_ex
+    `{CC : Countable PreAct} `{@gLts P A H, !FiniteImagegLts P A}
+    `{@FinitaryAbsAction P T FinA PreAct A H Φ 𝝳 _ gLtsT _ _ }
+    (p : P) pt G s hcnv :
 
     pt ∈ AFTER p s hcnv 
-    -> ~ MUST pt (union_of_actions_without ((elements (wt_refuses_set p s hcnv)) , q')) ->
-    exists p', pt ⟹ p' /\ p' ↛ /\ lts_acc_set_of p' ⊆ lts_acc_set_of q'.
+    -> ~ pt MUST ((oas p s hcnv) ∖ G) ->
+    exists p', pt ⟹ p' /\ p' ↛ /\ (coR_abs p') ⊆ G.
   Proof.
     intros mem%wt_set_spec1 hnm.
     eapply nMust_ex in hnm as (p' & hw' & nhw).
-    assert (ht': p' ⤓)
+    + assert (ht': p' ⤓)
       by (eapply (cnv_wt_s_terminate p p' s hcnv), wt_push_nil_right; eauto).
-    eapply terminate_then_wt_refuses in ht' as (p0 & hw0 & hst).
-    exists p0. split. eapply wt_push_nil_left; eauto.
-    split; eauto.
-    intros μ mem_mu.
-    assert (mem0 : μ ∈ actions_acc p s hcnv).
-    eapply elem_of_union_list. eexists. split; eauto.
-    eapply list_elem_of_fmap.
-    exists p0. repeat split; eauto.
-    eapply elem_of_elements, wt_refuses_set_spec2; split; eauto.
-    eapply wt_push_nil_right, wt_push_nil_right; eauto.
-    eapply lts_refuses_spec1 in mem_mu as (p'0 & HypTr).
-    { destruct (decide (μ ∈ lts_acc_set_of q')).
-      + eauto.
-      + exfalso.
-        eapply (nhw $ μ); eauto. unfold actions_acc in mem0.
-        unfold oas in mem0. set_solver.
-        eapply wt_push_nil_left; eauto with mdb. }
-    constructor; eapply (cnv_wt_s_terminate p pt s hcnv); eauto.
-  Qed. *)
+      eapply terminate_then_wt_refuses in ht' as (p0 & hw0 & hst).
+      exists p0. split. eapply wt_push_nil_left; eauto.
+      split; eauto.
+      intros pre_μ mem_mu.
+      assert (mem0 : pre_μ ∈ oas p s hcnv).
+      { eapply elem_of_union_list. eexists. split; eauto.
+        eapply list_elem_of_fmap.
+        exists p0. repeat split; eauto.
+        eapply elem_of_elements, wt_refuses_set_spec2; split; eauto.
+        eapply wt_push_nil_right, wt_push_nil_right; eauto. }
+      (* eapply lts_refuses_spec1 in mem_mu as (p'0 & HypTr). *)
+      { destruct (decide (pre_μ ∈ G)).
+        + eauto.
+        + exfalso. 
+          eapply coR_abs_spec1 in mem_mu as Hyp.
+          destruct Hyp as (μ & Hyp_co & eq). subst.
+          destruct Hyp_co as (μ' & tr & duo & b).
+          symmetry in duo. eapply unique_nb in duo as eq. eapply lts_refuses_spec1 in tr as (p'' & tr'').
+          eapply (nhw $ μ); eauto.
+          unfold oas in mem0. set_solver.
+          rewrite eq in tr''. eapply wt_push_nil_left; eauto with mdb. }
+     + constructor; eapply (cnv_wt_s_terminate p pt s hcnv); eauto.
+  Qed.
 
-(*   Lemma either_MUST_or_ex 
-    (p : P * mb A) (q' : Q * mb A)  s hcnv :
-    MUST__s (AFTER p s hcnv) (union_of_actions_without ((elements (wt_refuses_set p s hcnv)) , q'))
-    \/ (exists p', p ⟹[s] p' /\ p' ↛ /\ lts_acc_set_of p' ⊆ lts_acc_set_of q').
+  Lemma either_MUST_or_ex
+    `{CC : Countable PreAct} `{@gLts P A H, !FiniteImagegLts P A}
+    `{@FinitaryAbsAction P T FinA PreAct A H Φ 𝝳 _ gLtsT _ _ }
+    (p : P) G s hcnv :
+    MUST__s (AFTER p s hcnv) ((oas p s hcnv) ∖ G)
+    \/ (exists p', p ⟹[s] p' /\ p' ↛ /\ (coR_abs p') ⊆ G).
   Proof.
     assert (h1 : forall p0, p0 ∈ AFTER p s hcnv → p0 ⇓ []).
     intros p0 mem0. eapply cnv_nil, cnv_wt_s_terminate; eauto.
     eapply (wt_set_spec1 _ _ _ _ mem0).
-    destruct (either_MUST__s (AFTER p s hcnv) ((elements (wt_refuses_set p s hcnv)) , q')) 
+    destruct (either_MUST__s (AFTER p s hcnv) ((oas p s hcnv) ∖ G))
         as [ |Hyp].
     + eauto.
     + left. eauto.
@@ -191,49 +227,67 @@ Section must_set_acc_set.
       eapply nMusts_ex in Hyp as (pt & mem & hnm); eauto.
       eapply nMust_out_acc_ex in hnm as (pt' & hw & hst & hsub); eauto.
       exists pt'. split; eauto. eapply wt_push_nil_right; eauto. now eapply wt_set_spec1 in mem.
-  Qed. *)
+  Qed.
 
-(*   Lemma Must_out_acc_npre 
-    (p : P * mb A) (q q' : Q * mb A) s hcnv :
+  Lemma Must_out_acc_npre `{CC : Countable PreAct} `{@gLts P A H, !FiniteImagegLts P A}
+    `{@FinitaryAbsAction P T FinA PreAct A H Φ 𝝳 _ gLtsT _ _ }
+    `{@gLts Q A H, !FiniteImagegLts Q A}
+    `{@FinitaryAbsAction Q T FinA PreAct A _ Φ 𝝳 _ gLtsT _ _ }
+    (p : P) (q q' : Q) s hcnv :
     q ⇓ s -> q ⟹[s] q' -> q' ↛ ->
-    MUST__s (AFTER p s hcnv) (actions_acc p s hcnv ∖ lts_acc_set_of q') ->
-    ~ p ≾₂ q.
+    MUST__s (AFTER p s hcnv) (oas p s hcnv ∖ coR_abs q') ->
+    ~ p ₂≾ₘᵤₛₜ q.
   Proof.
     intros hcnv' hw hst hm pre2.
-    set (G := actions_acc p s hcnv ∖ lts_acc_set_of q').
-    assert (exists μ t, μ ∈ G /\ q' ⟹{μ} t) as (μ & t & mem & hw').
-    eapply (pre2 s hcnv hcnv'); eauto. eapply wt_set_spec2; eauto. eapply wt_nil.
+    set (G := (oas p s hcnv ∖ coR_abs q')).
+    assert (exists β t, (𝝳 ∘ Φ) β ∈ G /\ q' ⟹{co β} t) as (β & t & mem & hw' ). (* /\ blocking β & b *)
+    { eapply (pre2 s hcnv hcnv'); eauto. eapply wt_set_spec2; eauto. eapply wt_nil. }
     eapply elem_of_difference in mem as (mem & nmem).
-    (* assert (exists p', p' ⟶[ μ ]).
-    assert (is_output μ) as (a & heq). *)
-    eapply elem_of_union_list in mem as (X & mem1 & mem2).
-    eapply list_elem_of_fmap in mem1 as (r & heq & mem1). subst.
-    (* eapply elem_of_map in mem2 as (a & heq & mem2). exists a. assumption. *)
-    assert { r' | r ⟶[ μ ] r'} as (r' & HypTr). eapply lts_refuses_spec1. eauto.
-    inversion hw'; subst.
-    eapply lts_refuses_spec2 in hst; eauto.
-    eapply nmem. eapply lts_refuses_spec2. eauto.
-  Qed. *)
+    
+    destruct (decide (non_blocking β)) as [nb | b].
+    + admit.
+    + eapply elem_of_union_list in mem as (X & mem1 & mem2).
+      eapply list_elem_of_fmap in mem1 as (r & heq & mem1). subst.
+      
+      eapply coR_abs_spec1 in mem2 as Hyp.
+      destruct Hyp as (μ2 & Hyp_co & eq).
+      destruct Hyp_co as (μ'2 & tr & duo & b').
+      symmetry in duo. eapply unique_nb in duo as eq'. subst.
+      
+      assert { r' | r ⟶[ co μ2 ] r'} as (r' & HypTr).
+      { eapply lts_refuses_spec1. eauto. }
+      inversion hw'; subst.
+      * eapply lts_refuses_spec2 in hst; eauto.
+      * eapply nmem.
+      
+        eapply coR_abs_spec2.
+        eapply map_gamma_of_action.
+        
+        exists (co β). repeat split.
+        - eapply lts_refuses_spec2. eauto.
+        - symmetry. eapply (proj2_sig (exists_dual β)).
+        - exact b.
+  Admitted.
 
   (* ************************************************** *)
 
-  Context `{@gLtsObaFB T A H gLtsEqT gLtsObaT, !FiniteImagegLts T A}.
-
-  Context `{CC : Countable PreAct}.
-
-  Context `{@FinitaryAbsAction P T FinA PreAct A H Φ 𝝳 _ _ _ _ }.
-  Context `{@FinitaryAbsAction Q T FinA PreAct A H Φ 𝝳 _ _ _ _ }.
-
-  Lemma equivalence_bhv_acc_mst2
+  Lemma equivalence_bhv_acc_mst2 `{CC : Countable PreAct} `{@gLts P A H, !FiniteImagegLts P A}
+    `{@FinitaryAbsAction P T FinA PreAct A H Φ 𝝳 _ gLtsT _ _ }
+    `{@gLts Q A H, !FiniteImagegLts Q A}
+    `{@FinitaryAbsAction Q T FinA PreAct A _ Φ 𝝳 _ gLtsT _ _ }
+    `{!gLtsCNenabled Q A}
     (p : P) (q : Q) :
-    (p, ∅) ≼₁ (q, ∅) -> (p, ∅) ≾₂ (q, ∅) <-> (p, ∅) ≼₂ (q, ∅).
+    p ≼₁ q -> p ₂≾ₘᵤₛₜ q <-> p ≼₂ q.
   Proof.
     intro hpre1.
     split.
     - intro hpre2. intros s q' hcnv hw hst.
-      (* edestruct (either_MUST_or_ex (p, ∅) q' s hcnv).
-      + exfalso. eapply Must_out_acc_npre; eauto with mdb.
-      + set_solver. *) admit.
+      edestruct (either_MUST_or_ex p (coR_abs q') s hcnv).
+      + exfalso. eapply (Must_out_acc_npre p q) in H4;eauto.
+      + destruct H4 as (p' & wt_tr & stable & sub). 
+        exists p'. repeat split; eauto. intros pre_μ mem.
+        eapply coR_abs_spec2 in mem. eapply sub in mem.
+        eapply coR_abs_spec1; eauto.
     - intro hpre2.
       intros s hcnv hcnv' G hm q' mem%wt_set_spec1 q0 hw.
       assert (exists r, q0 ⟹ r /\ r ↛) as (qt & hw' & hstq').
@@ -241,44 +295,153 @@ Section must_set_acc_set.
         eapply cnv_wt_s_terminate; eauto. }
       edestruct (hpre2 s qt hcnv) as (pt & hwpt & hstpt & hsubpt); eauto.
       eapply wt_push_nil_right; eauto. eapply wt_push_nil_right; eauto.
-      assert (exists μ r, μ ∈ G /\ pt ⟹{μ} r) as (μ & p0 & mem0 & hw0).
+      assert (exists μ r, ( 𝝳 ∘ Φ ) μ ∈ G /\ pt ⟹{co μ} r) as (μ & p0 & mem0 & hw0).
       { eapply hm. eapply wt_set_spec2; eauto. eapply wt_nil. }
-      exists μ. inversion hw0; subst.
+      inversion hw0; subst.
       + exfalso. eapply lts_refuses_spec2 in hstpt; eauto.
-      + (* assert (𝝳 (Φ μ) ∈ coR_abs qt).
-        { eapply hsubpt. eapply preactions_of_spec. eapply preactions_of_fin_test_spec1.
-          admit. } *) admit.
-        (* exists qr. split; eauto. eapply wt_push_nil_left; eauto with mdb. *)
-  Admitted.
-
-  Theorem equivalence_bhv_acc_mst
-  (p : P) (q : Q) :
-  (p, ∅) ≾ₘᵤₛₜ (q, ∅) <-> (p, ∅) ≼ₐₛ (q, ∅).
-  Proof.
-    split; intros (pre1 & pre2); split; eauto; now eapply equivalence_bhv_acc_mst2.
+     
+      + destruct (decide (non_blocking μ)) as [nb | b].
+      
+        * assert (dual (co μ) μ) as duo.
+          { symmetry. eapply (proj2_sig (exists_dual μ)). }
+        
+          exists μ. destruct (cn_enabled q0 μ (co μ)) as (q'' & Hyp);eauto.
+          
+          exists q''. split; eauto. eapply lts_to_wt;eauto.
+          
+        * assert (( 𝝳 ∘ Φ) μ ∈ coR_abs qt) as mem'.
+          { eapply coR_abs_spec2. eapply hsubpt.
+          eapply map_gamma_of_action. exists (co μ).
+          repeat split.
+          -- eapply lts_refuses_spec2 ;eauto.
+          -- symmetry. eapply (proj2_sig (exists_dual μ)). 
+          -- exact b. }
+             eapply coR_abs_spec1 in mem'. destruct mem' as (μ' & mem' & eq).
+             destruct mem' as (μ'' & tr & duo & b').
+             exists μ'. eapply lts_refuses_spec1 in tr as (qr & tr_qr).
+             exists qr. split.
+             ++ rewrite<- eq; eauto.
+             ++ symmetry in duo. eapply unique_nb in duo. subst.
+                eapply wt_push_nil_left; eauto with mdb.
   Qed.
 
+Theorem equivalence_bhv_acc_mst_fw `{CC : Countable PreAct} `{
+  gLtsEqP : @gLtsEq P A H, !FiniteImagegLts P A,
+  gLtsEqQ : @gLtsEq Q A H, !FiniteImagegLts Q A, gLtsObaQ : !gLtsOba Q, !gLtsObaFW Q A,
+  FinAbsPT : @FinitaryAbsAction P T FinA PreAct A H Φ 𝝳 _ gLtsT _ _,
+  FinAbsQT : @FinitaryAbsAction Q T FinA PreAct A H Φ 𝝳 _ gLtsT _ _}
+  (p : P) (q : Q) :
+  p ≾ₘᵤₛₜ q <-> p ≼ₐₛ q.
+  Proof.
+    split; intros (pre1 & pre2) ; split; eauto; eapply equivalence_bhv_acc_mst2;eauto.
+    Unshelve.
+    eapply MkgLtsCNenabled. intros.
+    destruct (boomerang p1 η β) as (t & l1 & l2) ; eauto.
+    eapply MkgLtsCNenabled. intros.
+    destruct (boomerang p1 η β) as (t & l1 & l2) ; eauto.
+  Qed.
+
+Theorem equivalence_bhv_acc_mst `{CC : Countable PreAct} `{
+  gLtsP : @gLtsEq P A H, !FiniteImagegLts P A, FinAbsPT : @FinitaryAbsAction P T FinA PreAct A H Φ 𝝳 _ gLtsT _ _,
+  gLtsQ : @gLtsEq Q A H, !FiniteImagegLts Q A, FinAbsQT : @FinitaryAbsAction Q T FinA PreAct A H Φ 𝝳 _ gLtsT _ _}
+  `{!gLtsCNenabled Q A}
+  (p : P) (q : Q) :
+  p ≾ₘᵤₛₜ q <-> p ≼ₐₛ q.
+  Proof.
+    split; intros (pre1 & pre2) ; split; eauto; eapply equivalence_bhv_acc_mst2;eauto.
+  Qed.
+
+From stdpp Require Import base decidable gmap finite.
+From Stdlib Require Import ssreflect.
+From Stdlib.Program Require Import Equality.
+From TestingTheory Require Import gLts Bisimulation Lts_OBA Lts_FW Lts_OBA_FB StateTransitionSystems Termination
+    Must Bar Completeness Soundness Lift Subset_Act FiniteImageLTS WeakTransitions Convergence
+    InteractionBetweenLts MultisetLTSConstruction ForwarderConstruction ParallelLTSConstruction ActTau
+    Testing_Predicate DefinitionAS MustE Lts_Finite_Output_Chain Equivalence Soundness Completeness.
+
+Section preorder.
   Context `{outcome : T -> Prop}.
   Context `{outcome_dec : forall t, Decision (outcome t)}.
+  Context `{P : Type}.
+  Context `{Q : Type}.
+  Context `{H : !ExtAction A}.
 
-  Context `{Testing_Predicate0 :!Testing_Predicate outcome _}.
+  Context `{@gLtsOba P A H gLtsEqP, !FiniteImagegLts P A}.
+  Context `{@gLtsOba Q A H gLtsEqQ, !FiniteImagegLts Q A}.
+  Context `{@gLtsOba T A H gLtsEqT, !FiniteImagegLts T A, !Testing_Predicate outcome _}.
 
   Context `{!Prop_of_Inter P T A dual}.
   Context `{!Prop_of_Inter Q T A dual}.
-  Context `{!Prop_of_Inter (P * mb A) T A dual}.
-  Context `{!Prop_of_Inter (Q * mb A) T A dual}.
 
-  Context `{igen_conv : @test_convergence_spec T _  _ _ outcome Testing_Predicate0 gen_conv}.
-  Context `{igen_acc : @test_co_acceptance_set_spec PreAct _ _ T _ _ _ outcome Testing_Predicate0 gen_acc (fun x => 𝝳 (Φ x))}.
+  Context `{!Prop_of_Inter P (MO A) A fw_inter}.
+  Context `{!Prop_of_Inter (P * MO A) T A dual}.
+  Context `{!Prop_of_Inter Q (MO A) A fw_inter}.
+  Context `{!Prop_of_Inter (Q * MO A) T A dual}.
 
-  Corollary equivalence_bhv_mst_ctx
-    (p : P) (q : Q) : (p, ∅) ≾ₘᵤₛₜ (q, ∅) <-> pre_extensional outcome p q.
+
+  Context `{CC : Countable PreAct}.
+  Context `{@FinitaryAbsAction P T FinA PreAct A H Φ 𝝳 _ _ _ _ }.
+  Context `{@FinitaryAbsAction Q T FinA PreAct A H Φ 𝝳 _ _ _ _ }.
+
+  Context `{tc_spec : @test_convergence_spec T _ _ _ outcome _ t_conv}.
+  Context `{ta_spec : @test_co_acceptance_set_spec PreAct _ _ T _ _ _ outcome Testing_Predicate0 ta (fun x => 𝝳 (Φ x))}.
+
+  (** * Main equivalence theorems *)
+
+  Section FWⁿ.
+
+  Context `{!gLtsObaFW P A}.
+  Context `{!gLtsObaFW Q A}.
+  Context `{!gLtsObaFB T A}.
+
+  (** ** The must-set characterisation on FW is equivalent to the extensional must preorder *)
+  Corollary equivalence_fw_must_set_and_must_e
+    (p : P) (q : Q) : p ≾ₘᵤₛₜ q <-> pre_extensional outcome p q.
   Proof.
-    erewrite pre_extensional_eq.
-    rewrite equivalence_bhv_acc_mst.
-    (* erewrite <- equivalence_bhv_acc_ctx.
-    eapply pre_extensional_eq. *) admit.
-  Admitted.
+    erewrite equivalence_fw_bhv_acc_ctx.
+    rewrite equivalence_bhv_acc_mst_fw;eauto.
+  Qed.
 
+  (** ** The must-set characterisation on FW is equivalent to the inductive must preorder *)
+  Corollary equivalence_fw_must_set_and_must_i (p : P) (q : Q) :
+    p ⊑ₘᵤₛₜᵢ q <-> p ≾ₘᵤₛₜ q.
+  Proof.
+    split.
+    - intros hpre. eapply completeness_fw in hpre.
+      now eapply equivalence_bhv_acc_mst_fw.
+    - intros hpre. eapply soundness_fw.
+      now eapply equivalence_bhv_acc_mst_fw.
+  Qed.
 
-End must_set_acc_set.
+  End FWⁿ.
+  (** ---- *)
+  Section Lⁿ.
+
+  Context `{!gLtsObaFB P A, !FiniteOutputChain_LtsOba P}.
+  Context `{!gLtsObaFB Q A, !FiniteOutputChain_LtsOba Q}.
+  Context `{!gLtsObaFB T A, !FiniteOutputChain_LtsOba T}.
+
+  (** ** The must-set characterisation on toFW is equivalent to the inductive must preorder *)
+  Corollary equivalence_must_set_and_must_i (p : P) (q : Q) :
+    p ⊑ₘᵤₛₜᵢ q <-> (p, ∅) ≾ₘᵤₛₜ (q, ∅).
+  Proof.
+    split.
+    - intros hpre. eapply equivalence_bhv_acc_mst_fw.
+      eapply lift_fw_ctx_pre , completeness_fw in hpre. eauto.
+    - intros hpre%equivalence_bhv_acc_mst_fw.
+      eapply lift_fw_ctx_pre.
+      eapply soundness_fw; eauto.
+  Qed.
+
+  (** ---- *)
+
+  (** ** The inductive characterisation on toFW is equivalent to the extensional must preorder *)
+  Corollary equivalence_must_set_and_must_e (p : P) (q : Q) :
+    pre_extensional outcome p q <-> (p, ∅) ≾ₘᵤₛₜ (q, ∅).
+  Proof.
+    rewrite pre_extensional_eq. apply equivalence_must_set_and_must_i.
+  Qed.
+
+  End Lⁿ.
+
+End preorder.
