theories/Testing_Pre_orders/Must/Alternative_Preorder/Acceptance_Set/Soundness.v
@@ -1083,7 +1083,7 @@ Qed.
 End SoundnessAS.
 
 Lemma soundness_co_nb_enabled `{
-  gLtsEqP : @gLtsEq P A H, !FiniteImagegLts P A,
+  gLtsP : @gLtsEq P A H, !FiniteImagegLts P A,
   gLtsQ : !gLtsEq Q H, !gLtsCNenabled Q A, !FiniteImagegLts Q A,
   gLtsT : !gLtsEq T H, !Testing_Predicate outcome _}
 
